WIP generalizing connection interface.

examples/conn/proofs/base.v
@@ -2,13 +2,15 @@ From stdpp Require Import base gmap.
 From mathcomp Require Import ssreflect.
 From stdpp Require Import namespaces coGset.
 From iris.algebra Require Import agree auth csum gset gmap excl frac numbers.
+From iris.algebra Require Import max_prefix_list.
+From iris.bi.lib Require Import fractional.
 From iris.base_logic.lib Require Import invariants.
 From iris.heap_lang Require Import notation proofmode.
 From iris.heap_lang.lib Require Import ticket_lock.
 From cryptis Require Import lib term gmeta nown.
 From cryptis Require Import cryptis primitives tactics role.
 From cryptis Require Import saved_prop.
-From cryptis.examples Require Import iso_dh.
+From cryptis.examples Require Import iso_dh gen_conn.
 
 Set Implicit Arguments.
 Unset Strict Implicit.
@@ -16,220 +18,94 @@ Unset Printing Implicit Defensive.
 
 Local Notation connN := (nroot.@"conn").
 
-Record state := State {
-  cs_si   :> sess_info;
-  cs_ts   :  loc;
-  cs_chan :  val;
-  cs_role :  role;
+Record params Σ := Params {
+  msg_inv : sign_key → sign_key → sess_info → role → term → iProp Σ;
 }.
-
-Definition cs_share cs := si_share_of (cs_role cs) cs.
-
-#[global]
-Instance cs_repr : Repr state :=
-  λ s, (#(cs_ts s), si_key s, cs_chan s, repr (cs_role s))%V.
-
-Definition countR := authR max_natUR.
-
-Class connGS Σ := ConnGS {
-  connGS_count  : inG Σ countR;
-  connGS_pred   : savedPredG Σ (sign_key * sign_key * sess_info * role * term);
-}.
-
-Local Existing Instance connGS_count.
-Local Existing Instance connGS_pred.
-
-Definition connΣ := #[
-  GFunctor countR;
-  savedPredΣ (sign_key * sign_key * sess_info * role * term)
-].
-
-Global Instance subG_connGS Σ : subG connΣ Σ → connGS Σ.
-Proof. solve_inG. Qed.
 
 Section Defs.
 
-Context `{!cryptisGS Σ, !heapGS Σ, !connGS Σ}.
+Context `{!cryptisGS Σ, !heapGS Σ, !GenConn.connGS Σ}.
 Notation iProp := (iProp Σ).
 
-Implicit Types (cs : state).
+Implicit Types (cs : GenConn.state).
 Implicit Types (kS t : term) (ts : list term).
 Implicit Types (skI skR : sign_key).
 Implicit Types n m : nat.
 Implicit Types b : bool.
 Implicit Types v : val.
 Implicit Types (ok : Prop) (failed : bool).
-Implicit Types si : sess_info.
-Implicit Types (φ : sign_key → sign_key → sess_info → role → term → iProp).
-Implicit Types (ψ : role → term → iProp).
+Implicit Types (si : sess_info) (rl : role).
+Implicit Types (ps : params Σ).
 
-Definition failure skI skR : iProp :=
-   public skI ∨ public skR.
+Definition gen_conn_params ps : GenConn.params Σ := {|
+  GenConn.init_state := True;
+  GenConn.resp_state := True;
+  GenConn.chan_inv := λ skI skR si tsI tsR,
+    ([∗ list] t ∈ tsI, msg_inv ps skI skR si Init t) ∗
+    ([∗ list] t ∈ tsR, msg_inv ps skI skR si Resp t);
+  GenConn.msg_inv := λ skI skR si rl t, msg_inv ps skI skR si (swap_role rl) t;
+|}%I.
 
-Definition wf_sess_info rl si : iProp :=
-  minted (si_key si) ∗
-  session rl si.
+Local Coercion gen_conn_params : params >-> GenConn.params.
 
-#[global]
-Instance wf_sess_info_persistent rl si : Persistent (wf_sess_info rl si).
-Proof. apply _. Qed.
+Definition connected ps skI skR rl cs : iProp :=
+  GenConn.connected ps skI skR rl cs.
 
-Definition never_connected skI skR : iProp :=
-  term_token skR (↑connN.@"server".@skI).
-
-Lemma never_connected_switch skI skR Q : ⊢ switch (never_connected skI skR) Q.
-Proof. apply term_token_switch. Qed.
-
-Definition received_auth si rl n : iProp :=
-  term_own (si_share_of rl si) (connN.@"received") (● MaxNat n).
-
-Definition received_frag si rl n : iProp :=
-  term_own (si_share_of rl si) (connN.@"received") (◯ MaxNat n).
-
-Lemma received_update si rl n :
-  received_auth si rl n ==∗
-  received_auth si rl (S n) ∗ received_frag si rl (S n).
-Proof.
-rewrite /received_auth /received_frag -term_own_op.
-iApply term_own_update.
-apply: auth_update_alloc.
-apply: max_nat_local_update => /=; lia.
-Qed.
-
-Lemma received_alloc si rl E :
-  ↑connN.@"received" ⊆ E →
-  term_token (si_share_of rl si) E ==∗
-  received_auth si rl 0 ∗
-  term_token (si_share_of rl si) (E ∖ ↑connN.@"received").
-Proof.
-iIntros "% token".
-iMod (term_own_alloc (connN.@"received") (● MaxNat 0)
-       with "token") as "[own token]" => //.
-- by rewrite auth_auth_valid.
-- by iFrame.
-Qed.
-
-Lemma escrow_received n P si rl :
-  P ={⊤}=∗
-  escrow nroot (received_auth si rl n) (P ∗ received_auth si rl (S n)).
-Proof.
-iIntros "P".
-iMod (inv_alloc nroot _ (P ∨ received_frag si rl (S n))%I with "[P]") as "#I".
-{ by eauto. }
-rewrite /escrow. iIntros "!> !> %E %sub recv".
-iInv nroot as "[HP|>recv']".
-- iMod (received_update with "recv") as "[recv #frag]".
-  iModIntro. iSplitR; iFrame; by eauto.
-- iPoseProof (term_own_valid_2 with "recv recv'") as "%valid".
-  rewrite auth_both_valid_discrete max_nat_included in valid.
-  case: valid => /= ? _; lia.
-Qed.
-
-Definition conn_msg_pred φ gb : iProp :=
-  □ (∀ si rl t,
-        term_pred gb (iso_dhN.@"res".@"pred")
-          (si_init si, si_resp si, si, rl, t)
-          ↔ ▷ φ (si_init si) (si_resp si) si rl t).
-
-Definition conn_init_pred φ ψ gb : iProp :=
-  conn_msg_pred φ gb ∗ ψ Init gb.
-
-Definition connected skI skR φ rl cs : iProp :=
-  ⌜si_init cs = skI⌝ ∗
-  ⌜si_resp cs = skR⌝ ∗
-  ⌜cs_role cs = rl⌝ ∗
-  channel (cs_chan cs) ∗
-  wf_sess_info (cs_role cs) cs ∗
-  (compromised_session rl cs ∨
-     conn_msg_pred φ (si_resp_share cs)) ∗
-  ∃ n m, cs_ts cs ↦∗ [ #n; #m ] ∗ received_auth cs (cs_role cs) m.
-
-Lemma connected_channel skI skR φ rl cs :
-  connected skI skR φ rl cs -∗
-  channel (cs_chan cs).
-Proof. by iIntros "(_ & _ & _ & ? & _)". Qed.
-
-Lemma connected_public_key skI skR φ rl cs :
-  connected skI skR φ rl cs -∗
+Lemma connected_public_key ps skI skR rl cs :
+  connected ps skI skR rl cs -∗
   release_token (si_share_of rl cs) -∗
   public (si_key cs) -∗
   ◇ compromised_session rl cs.
-Proof.
-iIntros "conn rel #p_k".
-iPoseProof "conn" as "(_ & _ & <- & _ & #sess & _)".
-iDestruct "sess" as "(#? & #sess)".
-by iApply (session_compromised with "[] [//] rel").
-Qed.
+Proof. exact: GenConn.connected_public_key. Qed.
 
-Lemma connected_released_session skI skR φ rl cs :
-  connected skI skR φ rl cs -∗
+Lemma connected_released_session ps skI skR rl cs :
+  connected ps skI skR rl cs -∗
   □ (▷ released_session cs → public (si_key cs)).
-Proof.
-iIntros "(_ & _ & _ & _ & #sess & _)".
-by iDestruct "sess" as "(_ & ? & sess)".
-Qed.
+Proof. exact: GenConn.connected_released_session. Qed.
 
-Lemma connected_keyE skI skR φ rl cs :
-  connected skI skR φ rl cs -∗
-  ⌜skI = si_init cs⌝ ∗ ⌜skR = si_resp cs⌝ ∗ ⌜rl = cs_role cs⌝.
-Proof. by iIntros "(-> & -> & -> & _)". Qed.
+Lemma connected_keyE ps skI skR rl cs :
+  connected ps skI skR rl cs -∗
+  ⌜skI = si_init cs⌝ ∗ ⌜skR = si_resp cs⌝ ∗ ⌜rl = GenConn.cs_role cs⌝.
+Proof. exact: GenConn.connected_keyE. Qed.
 
-Lemma connected_ok skI skR φ rl cs :
-  connected skI skR φ rl cs -∗
+Lemma connected_ok ps skI skR rl cs :
+  connected ps skI skR rl cs -∗
   secret skI -∗
   secret skR -∗
   minted skI -∗
   minted skR -∗
   ◇ □ ¬ compromised_session rl cs.
-Proof.
-iIntros "(<- & <- & <- & _ & #sess & _ & % & % & _ & _)
-          s_kI s_kR #signI #signR".
-iDestruct "sess" as "(m_k & sess)".
-by iApply (session_not_compromised with "[//] s_kI s_kR").
-Qed.
-
-Definition conn_pred kS t : iProp :=
-  ∃ si rl n t',
-    let rl' := TInt (if rl is Init then 1 else 0) in
-    ⌜kS = si_key si⌝ ∗
-    ⌜t = Spec.of_list [rl'; TInt n; t']⌝ ∗
-    public t' ∗
-    escrow nroot (received_auth si (swap_role rl) n)
-      (term_pred (si_resp_share si) (iso_dhN.@"res".@"pred")
-         (si_init si, si_resp si, si, rl, t')
-       ∗ received_auth si (swap_role rl) (S n)).
+Proof. exact: GenConn.connected_ok. Qed.
 
 Lemma session_failed_failure rl si :
-  compromised_session rl si  ⊢ failure (si_init si) (si_resp si).
-Proof. by iIntros "(#failed & _)". Qed.
+  compromised_session rl si  ⊢ GenConn.failure (si_init si) (si_resp si).
+Proof. exact: GenConn.session_failed_failure. Qed.
+
+Lemma connected_failure ps skI skR rl cs :
+  connected ps skI skR rl cs -∗
+  release_token (si_share_of rl cs) -∗
+  public (si_key cs) -∗
+  ◇ GenConn.failure skI skR.
+Proof. exact: GenConn.connected_failure. Qed.
 
 Definition pre_ctx `{!iso_dhGS Σ} : iProp :=
-  iso_dh_ctx ∗
-  senc_pred connN conn_pred.
+  GenConn.pre_ctx.
 
 Lemma pre_ctx_alloc `{!iso_dhGS Σ} E :
   ↑connN ⊆ E →
   iso_dh_ctx -∗
   seal_pred_token SENC E ==∗
   pre_ctx ∗ seal_pred_token SENC (E ∖ ↑connN).
-Proof.
-iIntros "% #? tok". iFrame "#". by iApply seal_pred_set.
-Qed.
+Proof. exact: GenConn.pre_ctx_alloc. Qed.
 
-Definition ctx `{!iso_dhGS Σ} N φ ψ : iProp :=
-  pre_ctx ∗
-  iso_dh_pred N (conn_init_pred φ ψ).
+Definition ctx `{!iso_dhGS Σ} N ps : iProp :=
+  GenConn.ctx N ps.
 
-Lemma ctx_alloc `{!iso_dhGS Σ} N φ ψ E :
+Lemma ctx_alloc `{!iso_dhGS Σ} N ps E :
   ↑N ⊆ E →
   pre_ctx -∗
   iso_dh_token E ==∗
-  ctx N φ ψ ∗ iso_dh_token (E ∖ ↑N).
-Proof.
-iIntros "% #ctx tok". iFrame "#".
-by iApply iso_dh_pred_set.
-Qed.
+  ctx N ps ∗ iso_dh_token (E ∖ ↑N).
+Proof. exact: GenConn.ctx_alloc. Qed.
 
 End Defs.
-
-Arguments connGS Σ : clear implicits.
