examples/conn.v
@@ -1,10 +1,9 @@
 From cryptis.examples Require Import iso_dh.
-From cryptis.examples.conn Require Import impl proofs.
+From cryptis.examples.gen_conn Require impl.
+From cryptis.examples.conn Require Import proofs.
 
 Module Conn.
-Include cryptis.examples.conn.impl.
+Include cryptis.examples.gen_conn.impl.
 Include cryptis.examples.conn.proofs.base.
 Include cryptis.examples.conn.proofs.
 End Conn.
-
-Coercion Conn.cs_si : Conn.state >-> sess_info.
