examples/conn/proofs.v
@@ -6,8 +6,7 @@ From iris.algebra Require Import max_prefix_list.
 From iris.base_logic.lib Require Import invariants.
 From iris.heap_lang Require Import notation proofmode.
 From cryptis Require Import lib term gmeta cryptis primitives tactics role.
-From cryptis.examples Require Import iso_dh.
-From cryptis.examples.conn Require impl.
+From cryptis.examples Require Import iso_dh gen_conn.
 From cryptis.examples.conn.proofs Require Import base.
 
 Set Implicit Arguments.
@@ -18,10 +17,10 @@ Local Notation connN := (nroot.@"conn").
 
 Section Proofs.
 
-Context `{!cryptisGS Σ, !heapGS Σ, !connGS Σ, !iso_dhGS Σ}.
+Context `{!cryptisGS Σ, !heapGS Σ, !GenConn.connGS Σ, !iso_dhGS Σ}.
 Notation iProp := (iProp Σ).
 
-Implicit Types (cs : state).
+Implicit Types (cs : GenConn.state).
 Implicit Types kS t : term.
 Implicit Types skI skR : sign_key.
 Implicit Types n m : nat.
@@ -29,273 +28,85 @@ Implicit Types γ : gname.
 Implicit Types v : val.
 Implicit Types (N : namespace).
 
-Lemma wp_channel cs :
-  {{{ True }}}
-    impl.channel (repr cs)
-  {{{ RET (cs_chan cs); True }}}.
-Proof.
-iIntros "% _ post". wp_lam. wp_pures. by iApply "post".
-Qed.
-
-Lemma wp_connect P c skI skR N φ ψ :
+Lemma wp_connect P c skI skR N ps :
   channel c ∗
   cryptis_ctx ∗
-  ctx N φ ψ ∗
+  ctx N ps ∗
   minted skI ∗
   minted skR -∗
-  {{{ (failure skI skR ∨ P) }}}
+  {{{ GenConn.failure skI skR ∨ P }}}
     impl.connect c skI (Spec.pkey skR) (Tag N)
   {{{ cs, RET (repr cs);
-      connected skI skR φ Init cs ∗
-      (compromised_session Init cs ∨ P ∗ ψ Init (si_resp_share cs)) ∗
+      connected ps skI skR Init cs ∗
+      (public (si_key cs) ∨ P) ∗
       release_token (si_init_share cs) ∗
       term_token (si_init_share cs) (⊤ ∖ ↑iso_dhN ∖ ↑connN) }}}.
-Proof.
-iIntros "(#? & #? & ([#? #?] & #?) & #? & #?) % !> HP post".
-rewrite bi.or_alt. iDestruct "HP" as "(%failed & HP)".
-wp_lam. wp_pure _ credit:"c1". wp_pure _ credit:"c2".
-wp_pures. wp_bind (do_until _).
-iAssert (if failed then failure skI skR else True)%I as "#?".
-{ by case: failed. }
-iCombine "HP post c1 c2" as "post". iApply (wp_frame_wand with "post").
-iApply wp_do_until'. iIntros "!>". wp_pures.
-wp_apply (wp_initiator failed with "[//] [//] [] [//] [] [] [] []") => //.
-iIntros "%res resP".
-case: res=> [kS|] /=; last by eauto.
-iDestruct "resP"
-  as "(%si & <- & %e_kR & <- & #m_kS & #sess & #comp & rel & token & res)".
-move: e_kR => <-.
-iRight. iExists _. iSplit => //.
-iIntros "(dis & post & c1 & c2)".
-wp_pures.
-wp_alloc ts as "ts"; try lia. wp_pures. rewrite /=.
-pose cs := State si ts c Init.
-iMod (received_alloc si Init with "token") as "[received token]";
-  first solve_ndisj.
-iApply ("post" $! cs).
-rewrite /conn_init_pred or_sep2.
-iDestruct "res" as "[res1 res2]".
-iModIntro. iFrame.
-iSplit.
-{ do 6!iSplit => //. }
-iSplitR "token"; last first.
-{ iApply (term_token_drop with "token"). solve_ndisj. }
-iDestruct "res2" as "[?|res2]"; eauto.
-case: failed; [|iRight]; iFrame.
-iLeft. by iApply "comp".
-Qed.
+Proof. exact: GenConn.wp_connect. Qed.
 
-Lemma wp_listen c N φ ψ :
+Lemma wp_listen c N ps :
   channel c -∗
   cryptis_ctx -∗
-  ctx N φ ψ -∗
+  ctx N ps -∗
   {{{ True }}}
     impl.listen c
   {{{ ga skI, RET (ga, Spec.pkey skI)%V;
       public ga ∗ minted skI }}}.
-Proof.
-iIntros "#? #? [[#? _] _] % !> _ post". wp_lam.
-wp_apply wp_responder_wait; eauto.
-Qed.
+Proof. exact: GenConn.wp_listen. Qed.
 
-Lemma wp_confirm P ψ c skI skR ga N φ :
-  channel c -∗
-  cryptis_ctx -∗
-  ctx N φ ψ -∗
+Lemma wp_confirm P ps c skI skR ga N :
+  channel c ∗
+  cryptis_ctx ∗
+  ctx N ps -∗
   {{{ public ga ∗ minted skI ∗ minted skR ∗
-      □ (∀ gb, term_token gb (↑iso_dhN.@"res" ∖ ↑iso_dhN.@"res".@"pred") ={⊤}=∗
-               ψ Init gb ∗ ψ Resp gb) ∗
-      (failure skI skR ∨ P) }}}
+      (GenConn.failure skI skR ∨ P) }}}
     impl.confirm c skR (Tag N) (ga, Spec.pkey skI)%V
   {{{ cs, RET (repr cs);
-      connected skI skR φ Resp cs ∗
-      (compromised_session Resp cs ∨ P) ∗
+      connected ps skI skR Resp cs ∗
+      (public (si_key cs) ∨ P) ∗
       release_token (si_resp_share cs) ∗
-      term_token (si_resp_share cs) (⊤ ∖ ↑iso_dhN ∖ ↑connN) ∗
-      ψ Resp (si_resp_share cs) }}}.
+      term_token (si_resp_share cs) (⊤ ∖ ↑iso_dhN ∖ ↑connN) }}}.
 Proof.
-iIntros "#? #ctx [[#? #?] #?] !> %Φ (#p_ga & #p_pkA & #sign_skB & #mk & P) post".
-rewrite bi.or_alt. iDestruct "P" as "(%failed & P)".
-wp_lam. wp_pures.
-iAssert (if failed then failure skI skR else True)%I
-  as "#?".
-{ by case: failed. }
-wp_bind (do_until _).
-iApply (wp_frame_wand with "post").
-iApply (wp_frame_wand with "P").
-iApply wp_do_until'. iIntros "!>".
-wp_pures.
-iApply (wp_responder_accept failed (λ gb, conn_msg_pred φ gb ∗ ψ Resp gb))%I.
-{ do !iSplit => //.
-  iIntros "%gb token".
-  iMod (term_pred_alloc _ (N := iso_dhN.@"res".@"pred")
-          (λ '(skI, skR, si, rl, t), φ skI skR si rl t) with "token")
-    as "[#pred token]"; try solve_ndisj.
-  iAssert (conn_msg_pred φ gb) as "#?".
-  { iModIntro. iIntros "% % %". iApply ("pred" $! (_, _, _)). }
-  iMod ("mk" with "token") as "[init resp]". iFrame. by eauto. }
-iIntros "!> %osi res". case: osi => [kS|]; last by eauto.
-iDestruct "res"
-  as "(%si & <- & <- & -> & #m_k & #sess & #comp & rel & token & msg & res)".
-iRight. iExists _. iSplit => //.
-iIntros "P post".
-wp_pures.
-wp_alloc ts as "ts"; first lia.
-wp_pures.
-iMod (received_alloc si Resp with "token") as "[received token]";
-  first solve_ndisj.
-iApply ("post" $! (State si ts c Resp)).
-iModIntro. iFrame. do 7?iSplit => //.
-iSplitR "token".
-{ case: failed; eauto. iLeft. by iApply "comp". }
-iApply (term_token_drop with "token"). solve_ndisj.
+iIntros "#? !> %Φ (#p_ga & #p_pkA & #sign_skB & P) post".
+wp_apply (GenConn.wp_confirm P with "[//] [$P]") => //.
+do !iSplit => //=. by eauto.
 Qed.
 
-Lemma wp_session_key cs :
-  {{{ True }}}
-    impl.session_key (repr cs)
-  {{{ RET (repr (si_key cs)); True }}}.
-Proof.
-rewrite /impl.session_key.
-iIntros "%Φ _ post". wp_pures. iApply "post".
-iModIntro. by iFrame.
-Qed.
-
-Lemma wp_role cs :
-  {{{ True }}}
-    impl.role (repr cs)
-  {{{ RET (repr (cs_role cs)); True }}}.
-Proof.
-iIntros "%Φ _ post". wp_lam. wp_pures. by iApply "post".
-Qed.
-
-Lemma wp_send skI skR rl cs t N φ ψ :
-  ctx N φ ψ -∗
+Lemma wp_send skI skR rl cs t N ps :
+  ctx N ps -∗
   public t -∗
-  {{{ connected skI skR φ rl cs ∗
-      (public (si_key cs) ∨ φ skI skR cs rl t) }}}
+  {{{ connected ps skI skR rl cs ∗
+      (public (si_key cs) ∨ msg_inv ps skI skR cs rl t) }}}
     impl.send (repr cs) t
-  {{{ RET #(); connected skI skR φ rl cs }}}.
+  {{{ RET #(); connected ps skI skR rl cs }}}.
 Proof.
-iIntros "[[_ #pred] _] #p_ts !> %Φ (conn & inv) post".
-iDestruct "conn"
-  as "(<- & <- & <- & #chan & #sess & #msg & %n & %m & counters & recv)".
-wp_lam. wp_pures.
-wp_apply wp_channel => //. iIntros "_". wp_pures.
-wp_lam. wp_pures.
-wp_apply wp_session_key => //. iIntros "_".
-wp_pures.
-wp_list.
-wp_apply (wp_load_offset with "counters") => //.
-iIntros "counters".
-wp_apply wp_tint. wp_list. wp_apply wp_role => //. iIntros "_".
-wp_apply wp_tint. wp_list. wp_term_of_list.
-set msg := Spec.of_list _.
-iAssert (public msg) as "#?".
-{ rewrite public_of_list /= !public_TInt. by eauto. }
-iAssert (|={⊤}=> (public (si_key cs) ∨ conn_pred (si_key cs) msg))%I
-  with "[inv]" as ">#p_t".
-{ iDestruct "inv" as "[#?|inv]"; first by eauto.
-  iDestruct "msg" as "[(_ & ? & _)|msg]"; eauto.
-  iSpecialize ("msg" with "inv").
-  iRight. iExists cs, (cs_role cs), n, t.
-  do 3!iSplitR => //.
-  by iApply escrow_received. }
-wp_pures. wp_apply wp_senc; eauto.
-- by iDestruct "sess" as "(?&?)".
-- by iDestruct "p_t" as "[p_t|inv_t]"; eauto.
-iIntros "% #?". wp_pures. wp_apply wp_send => //. wp_pures.
-wp_apply (wp_load_offset with "counters") => //.
-iIntros "counters". wp_pures.
-wp_apply (wp_store_offset with "counters") => //=.
-rewrite (_ : (_ + _)%Z = S n); last by lia.
-iIntros "counters". iApply "post". iFrame. by eauto 10.
+iIntros "#ctx #p_t !> %Φ (conn & inv) post".
+wp_apply (GenConn.wp_send with "[//] [//] [$conn inv]") => //.
+iDestruct "inv" as "[fail|inv]"; auto.
+iRight. iIntros "% % [inv1 inv2]".
+by case: rl; iFrame; eauto.
 Qed.
 
-Ltac recv_failure :=
-  iLeft; iFrame; eauto 10.
-
-Lemma wp_recv skI skR rl cs N φ ψ :
-  ctx N φ ψ -∗
-  {{{ connected skI skR φ rl cs }}}
+Lemma wp_recv skI skR rl cs N ps :
+  ctx N ps -∗
+  {{{ connected ps skI skR rl cs }}}
     impl.recv (repr cs)
   {{{ t, RET (repr t);
-      connected skI skR φ rl cs ∗
+      connected ps skI skR rl cs ∗
       public t ∗
-      (public (si_key cs) ∨ φ skI skR cs (swap_role rl) t) }}}.
+      (public (si_key cs) ∨ msg_inv ps skI skR cs (swap_role rl) t) }}}.
 Proof.
-iIntros "[[_ #Nφ] _] !> %Φ conn post".
-wp_lam.
-iPoseProof (connected_channel with "conn") as "#?".
-wp_apply wp_channel => //. iIntros "_". wp_pures.
-wp_apply wp_role => //. iIntros "_". wp_pures.
-wp_apply wp_session_key => //. iIntros "_". wp_pures.
-iApply (wp_frame_wand with "post").
-iRevert "conn". iApply wp_do_until.
-iIntros "!> conn". wp_pure _ credit:"c1".
-wp_apply wp_recv => //. iIntros "%t #p_t". wp_pure _ credit:"c2". wp_pures.
-iDestruct "conn"
-  as "(<- & <- & <- & #chan & #sess & #msg & %n & %m & counters & recv)".
-wp_lam. wp_pures. wp_apply wp_sdec => //. iSplit; last first.
-{ wp_pures. iLeft. iFrame. by eauto 10. }
-iClear "p_t" => {t}. iIntros "%t #m_t #inv_t #s_t". wp_pures.
-wp_list_of_term t; wp_pures; last by recv_failure.
-wp_list_match => [rl' r' {}t ->|_]; wp_pures; last by recv_failure.
-wp_apply wp_to_int.
-case: Spec.to_intP => [ {}rl' ->|_]; wp_pures; last by recv_failure.
-wp_apply wp_to_int.
-case: Spec.to_intP => [ {}r' ->|_]; wp_pures; last by recv_failure.
-case: bool_decide_reflect => [?|ne]; wp_pures; first by recv_failure.
-wp_apply (wp_load_offset with "counters") => //. iIntros "counters".
-wp_pures. case: bool_decide_reflect => [[<-]|_]; wp_pures; last by recv_failure.
-wp_apply (wp_load_offset with "counters") => //. iIntros "counters".
-wp_pures. rewrite (_ : (m + 1)%Z = S m); last by lia.
-wp_apply (wp_store_offset with "counters") => //=. iIntros "counters".
-iAssert (|={⊤}=> public t ∗
-           received_auth cs (cs_role cs) (S m) ∗
-           (public (si_key cs) ∨
-              φ (si_init cs) (si_resp cs) cs (swap_role (cs_role cs)) t))%I
-  with "[recv c1 c2]" as "{inv_t} >(p_t & recv & inv_t)".
-{ iDestruct "inv_t" as "[fail|#inv]".
-  { iMod (received_update with "recv") as "[recv _]".
-    iDestruct ("s_t" with "fail") as "p_t".
-    rewrite public_of_list /=. iDestruct "p_t" as "(_ & _ & p_t & _)".
-    iFrame. by eauto. }
-  iDestruct "inv" as "(%si & %rl'' & %m' & %t' & %e_k & %e_t & p_ts & inv)".
-  move/term_of_senc_key_inj/session_agree: e_k => <- {si}.
-  case/Spec.of_list_inj: e_t => -> e_m <- {rl'} in ne *.
-  have <-: m = m' by lia.
-  have {ne} -> : rl'' = swap_role (cs_role cs).
-    rewrite /repr_role in ne.
-    case: rl'' (cs_role cs) => [] [] /= in ne *; congruence.
-  rewrite swap_roleK.
-  iMod (escrowE with "inv recv") as "{inv} [inv recv]";
-    first by solve_ndisj.
-  iFrame.
-  iCombine "inv recv" as "I".
-  iMod (lc_fupd_elim_later with "c1 I") as "[inv recv]".
-  iFrame. iSplitR; eauto.
-  iDestruct "msg" as "[(_ & ? & _)|msg]"; eauto.
-  iSpecialize ("msg" with "inv").
-  iMod (lc_fupd_elim_later with "c2 msg") as "msg".
-  by eauto. }
-wp_pures. iModIntro. iRight. iExists _. iSplit => //.
-iIntros "post". iApply "post". iFrame. by eauto 10.
+iIntros "#ctx !> %Φ conn post".
+wp_apply (GenConn.wp_recv with "[//] [$conn]") => //.
+iRight. iIntros "% % % [inv1 inv2]". rewrite/=.
+case: rl => /=; iFrame.
+- iDestruct "inv2" as "[??]". by iFrame.
+- iDestruct "inv1" as "[??]". by iFrame.
 Qed.
 
-Lemma wp_free kI kR φ rl cs :
-  {{{ connected kI kR φ rl cs }}}
+Lemma wp_free ps kI kR rl cs :
+  {{{ connected ps kI kR rl cs }}}
     impl.free (repr cs)
   {{{ RET #(); True }}}.
-Proof.
-iIntros "%Φ conn post".
-iDestruct "conn" as "(? & ? & ? & ? & ? & ? & % & % & ts & ?)".
-rewrite !array_cons array_nil.
-iDestruct "ts" as "(sent & recv & _)".
-wp_lam; wp_pures.
-wp_free. wp_pures.
-wp_free.
-by iApply "post".
-Qed.
+Proof. exact: GenConn.wp_free. Qed.
 
 End Proofs.
