examples/gen_conn.v
@@ -1,0 +1,10 @@
+From cryptis.examples Require Import iso_dh.
+From cryptis.examples.gen_conn Require Import impl proofs.
+
+Module GenConn.
+Include cryptis.examples.gen_conn.impl.
+Include cryptis.examples.gen_conn.proofs.base.
+Include cryptis.examples.gen_conn.proofs.
+End GenConn.
+
+Coercion GenConn.cs_si : GenConn.state >-> sess_info.
