examples/gen_conn/proofs.v
@@ -1,0 +1,309 @@
+From stdpp Require Import base gmap.
+From mathcomp Require Import ssreflect.
+From stdpp Require Import namespaces.
+From iris.algebra Require Import agree auth csum gset gmap excl frac.
+From iris.algebra Require Import max_prefix_list.
+From iris.base_logic.lib Require Import invariants.
+From iris.heap_lang Require Import notation proofmode.
+From cryptis Require Import lib term gmeta cryptis primitives tactics role.
+From cryptis.examples Require Import iso_dh.
+From cryptis.examples.gen_conn Require impl.
+From cryptis.examples.gen_conn.proofs Require Import base.
+
+Set Implicit Arguments.
+Unset Strict Implicit.
+Unset Printing Implicit Defensive.
+
+Local Notation connN := (nroot.@"conn").
+
+Section Proofs.
+
+Context `{!cryptisGS Σ, !heapGS Σ, !connGS Σ, !iso_dhGS Σ}.
+Notation iProp := (iProp Σ).
+
+Implicit Types (cs : state).
+Implicit Types kS t : term.
+Implicit Types skI skR : sign_key.
+Implicit Types n m : nat.
+Implicit Types γ : gname.
+Implicit Types v : val.
+Implicit Types (N : namespace).
+
+Lemma wp_channel cs :
+  {{{ True }}}
+    impl.channel (repr cs)
+  {{{ RET (cs_chan cs); True }}}.
+Proof.
+iIntros "% _ post". wp_lam. wp_pures. by iApply "post".
+Qed.
+
+Lemma wp_connect P c skI skR N ps :
+  channel c ∗
+  cryptis_ctx ∗
+  ctx N ps ∗
+  minted skI ∗
+  minted skR -∗
+  {{{ (failure skI skR ∨ P) }}}
+    impl.connect c skI (Spec.pkey skR) (Tag N)
+  {{{ cs, RET (repr cs);
+      connected ps skI skR Init cs ∗
+      (public (si_key cs) ∨ P) ∗
+      release_token (si_init_share cs) ∗
+      term_token (si_init_share cs) (⊤ ∖ ↑iso_dhN ∖ ↑connN) }}}.
+Proof.
+iIntros "(#? & #? & ([#? #?] & #?) & #? & #?) % !> HP post".
+rewrite bi.or_alt. iDestruct "HP" as "(%failed & HP)".
+wp_lam. wp_pure _ credit:"c1". wp_pure _ credit:"c2".
+wp_pures. wp_bind (do_until _).
+iAssert (if failed then failure skI skR else True)%I as "#?".
+{ by case: failed. }
+iCombine "HP post c1 c2" as "post". iApply (wp_frame_wand with "post").
+iApply wp_do_until'. iIntros "!>". wp_pures.
+wp_apply (wp_initiator failed with "[//] [//] [] [//] [] [] [] []") => //.
+iIntros "%res resP".
+case: res=> [kS|] /=; last by eauto.
+iDestruct "resP"
+  as "(%si & <- & %e_kR & <- & #m_kS & #sess & #comp & rel & token & res)".
+move: e_kR => <-.
+iRight. iExists _. iSplit => //.
+iIntros "(dis & post & c1 & c2)".
+wp_pures.
+wp_alloc ts as "ts"; try lia. wp_pures. rewrite /=.
+pose cs := State si ts c Init.
+iApply ("post" $! cs).
+iModIntro. iFrame.
+iSplit.
+{ do 6!iSplit => //. }
+iSplitR "token"; last first.
+{ iApply (term_token_drop with "token"). solve_ndisj. }
+case: failed; [|iRight]; iFrame.
+iLeft. by iApply "comp".
+Qed.
+
+Lemma wp_listen c N ps :
+  channel c -∗
+  cryptis_ctx -∗
+  ctx N ps -∗
+  {{{ True }}}
+    impl.listen c
+  {{{ ga skI, RET (ga, Spec.pkey skI)%V;
+      public ga ∗ minted skI }}}.
+Proof.
+iIntros "#? #? [[#? _] _] % !> _ post". wp_lam.
+wp_apply wp_responder_wait; eauto.
+Qed.
+
+Lemma wp_confirm P ps c skI skR ga N :
+  channel c ∗
+  cryptis_ctx ∗
+  ctx N ps -∗
+  {{{ public ga ∗ minted skI ∗ minted skR ∗
+      □ (∀ b,
+          let gb := TExp (TInt 0) b in
+          let gab := TExp ga b in
+          let si := SessInfo skI skR ga gb gab in
+          term_token (si_resp_share si)
+            (↑iso_dhN.@"res" ∖ ↑iso_dhN.@"res".@"chan") ={⊤}=∗
+            chan_inv ps skI skR si [] []) ∗
+      (failure skI skR ∨ P) }}}
+    impl.confirm c skR (Tag N) (ga, Spec.pkey skI)%V
+  {{{ cs, RET (repr cs);
+      connected ps skI skR Resp cs ∗
+      (public (si_key cs) ∨ P) ∗
+      release_token (si_resp_share cs) ∗
+      term_token (si_resp_share cs) (⊤ ∖ ↑iso_dhN ∖ ↑connN) }}}.
+Proof.
+iIntros "(#? & #ctx & [[#? #?] #?])".
+iIntros "!> %Φ (#p_ga & #p_pkA & #sign_skB & #mk & P) post".
+rewrite bi.or_alt. iDestruct "P" as "(%failed & P)".
+wp_lam. wp_pures.
+iAssert (if failed then failure skI skR else True)%I
+  as "#?".
+{ by case: failed. }
+wp_bind (do_until _).
+iApply (wp_frame_wand with "post").
+iApply (wp_frame_wand with "P").
+iApply wp_do_until'. iIntros "!>".
+wp_pures. iApply (wp_responder_accept failed).
+{ do !iSplit => //=.
+  iIntros "%gb token".
+  rewrite (term_token_difference _ (↑iso_dhN.@"res".@"chan"));
+    last solve_ndisj.
+  iDestruct "token" as "[chan token]".
+  iMod ("mk" with "token") as "inv".
+  set si := SessInfo _ _ _ _ _.
+  iMod (counters_alloc _ _ _ si with "chan inv") as "[c1 c2]".
+  by iFrame. }
+iIntros "!> %osi res". case: osi => [kS|]; last by eauto.
+iDestruct "res"
+  as "(%si & <- & <- & -> & #m_k & #sess & #comp & rel & token & res)".
+iRight. iExists _. iSplit => //.
+iIntros "P post".
+wp_pures.
+wp_alloc ts as "ts"; first lia.
+wp_pures.
+iApply ("post" $! (State si ts c Resp)).
+iModIntro. iFrame. rewrite /=. do 7?iSplit => //.
+iSplitR "token".
+{ case: failed; eauto. iLeft. by iApply "comp". }
+iApply (term_token_drop with "token"). solve_ndisj.
+Qed.
+
+Lemma wp_session_key cs :
+  {{{ True }}}
+    impl.session_key (repr cs)
+  {{{ RET (repr (si_key cs)); True }}}.
+Proof.
+rewrite /impl.session_key.
+iIntros "%Φ _ post". wp_pures. iApply "post".
+iModIntro. by iFrame.
+Qed.
+
+Lemma wp_role cs :
+  {{{ True }}}
+    impl.role (repr cs)
+  {{{ RET (repr (cs_role cs)); True }}}.
+Proof.
+iIntros "%Φ _ post". wp_lam. wp_pures. by iApply "post".
+Qed.
+
+Lemma wp_send skI skR rl cs t N ps :
+  ctx N ps -∗
+  public t -∗
+  {{{ connected ps skI skR rl cs ∗
+      (public (si_key cs) ∨
+         (∀ ts_send ts_recv,
+            ▷ chan_inv_for ps skI skR cs rl ts_send ts_recv ={⊤ ∖ ↑connN}=∗
+            ▷ chan_inv_for ps skI skR cs rl (ts_send ++ [t]) ts_recv)) }}}
+    impl.send (repr cs) t
+  {{{ RET #(); connected ps skI skR rl cs }}}.
+Proof.
+iIntros "[[_ #pred] _] #p_ts !> %Φ (conn & inv) post".
+iDestruct "conn"
+  as "(<- & <- & <- & #chan & #sess & %n & %m & state & counters)".
+wp_lam. wp_pures.
+wp_apply wp_channel => //. iIntros "_". wp_pures.
+wp_lam. wp_pures.
+wp_apply wp_session_key => //. iIntros "_".
+wp_pures.
+wp_list.
+wp_apply (wp_load_offset with "state") => //.
+iIntros "state".
+wp_apply wp_tint. wp_list. wp_apply wp_role => //. iIntros "_".
+wp_apply wp_tint. wp_list. wp_term_of_list.
+set msg := Spec.of_list _.
+iAssert (public msg) as "#?".
+{ rewrite public_of_list /= !public_TInt. by eauto. }
+iAssert (|={⊤}=>
+  (public (si_key cs) ∨
+     counters ps (si_init cs) (si_resp cs) cs (cs_role cs) (S n) m ∗
+     conn_msg_pred (si_key cs) msg))%I
+  with "[counters inv]" as ">inv".
+{ iDestruct "counters" as "[#fail|counters]"; first by eauto.
+  iDestruct "inv" as "[#?|inv]"; first by eauto.
+  iMod (counters_send with "counters inv") as "[#sent_at counters]".
+  iRight. iFrame. iExists cs, (cs_role cs), n, t.
+  do 3!iSplitR => //. }
+rewrite or_sep2. iDestruct "inv" as "[counters #p_t]".
+wp_pures. wp_apply wp_senc; eauto.
+- by iDestruct "sess" as "(?&?)".
+- by iDestruct "p_t" as "[p_t|inv_t]"; eauto.
+iIntros "% #?". wp_pures. wp_apply wp_send => //. wp_pures.
+wp_apply (wp_load_offset with "state") => //.
+iIntros "state". wp_pures.
+wp_apply (wp_store_offset with "state") => //=.
+rewrite (_ : (_ + _)%Z = S n); last by lia.
+iIntros "state". iApply "post". iFrame. by eauto 10.
+Qed.
+
+Ltac recv_failure :=
+  iLeft; iFrame; eauto 10.
+
+Lemma wp_recv skI skR rl cs N ps :
+  ctx N ps -∗
+  {{{ connected ps skI skR rl cs ∗
+      (public (si_key cs) ∨
+        (∀ t ts_send ts_recv,
+          ▷ chan_inv_for ps skI skR cs rl ts_send (t :: ts_recv) ={⊤ ∖ ↑connN}=∗
+          ▷ chan_inv_for ps skI skR cs rl ts_send ts_recv ∗
+          ▷ msg_inv ps skI skR cs rl t)) }}}
+    impl.recv (repr cs)
+  {{{ t, RET (repr t);
+      connected ps skI skR rl cs ∗
+      public t ∗
+      (public (si_key cs) ∨ msg_inv ps skI skR cs rl t) }}}.
+Proof.
+iIntros "[[_ #Nφ] _] !> %Φ (conn & recv) post".
+wp_lam.
+iPoseProof (connected_channel with "conn") as "#?".
+wp_apply wp_channel => //. iIntros "_". wp_pures.
+wp_apply wp_role => //. iIntros "_". wp_pures.
+wp_apply wp_session_key => //. iIntros "_". wp_pures.
+iApply (wp_frame_wand with "post").
+iCombine "conn recv" as "I". iRevert "I". iApply wp_do_until.
+iIntros "!> (conn & recv)". wp_pure _ credit:"c1".
+wp_apply wp_recv => //. iIntros "%t #p_t". wp_pure _ credit:"c2". wp_pures.
+iDestruct "conn"
+  as "(<- & <- & <- & #chan & #sess & %n & %m & state & counters)".
+wp_lam. wp_pures. wp_apply wp_sdec => //. iSplit; last first.
+{ wp_pures. iLeft. iFrame. by eauto 10. }
+iClear "p_t" => {t}. iIntros "%t #m_t #inv_t #s_t". wp_pures.
+wp_list_of_term t; wp_pures; last by recv_failure.
+wp_list_match => [rl' r' {}t ->|_]; wp_pures; last by recv_failure.
+wp_apply wp_to_int.
+case: Spec.to_intP => [ {}rl' ->|_]; wp_pures; last by recv_failure.
+wp_apply wp_to_int.
+case: Spec.to_intP => [ {}r' ->|_]; wp_pures; last by recv_failure.
+case: bool_decide_reflect => [?|ne]; wp_pures; first by recv_failure.
+wp_apply (wp_load_offset with "state") => //. iIntros "state".
+wp_pures. case: bool_decide_reflect => [[<-]|_]; wp_pures; last by recv_failure.
+wp_apply (wp_load_offset with "state") => //. iIntros "state".
+wp_pures. rewrite (_ : (m + 1)%Z = S m); last by lia.
+wp_apply (wp_store_offset with "state") => //=. iIntros "state".
+iAssert (public (si_key cs) → public t)%I as "{s_t} s_t".
+{ iIntros "#fail".
+  iDestruct ("s_t" with "fail") as "p_t".
+  rewrite public_of_list /=. by iDestruct "p_t" as "(_ & _ & p_t & _)". }
+iAssert (|={⊤}=>
+  public t ∗
+  (public (si_key cs) ∨
+    counters ps (si_init cs) (si_resp cs) cs (cs_role cs) n (S m) ∗
+    msg_inv ps (si_init cs) (si_resp cs) cs (cs_role cs) t))%I
+  with "[counters recv c1 c2]" as "{inv_t} >(p_t & inv)".
+{ iDestruct "recv" as "[#fail|recv]".
+  { iModIntro. iSplitR; eauto. by iApply "s_t". }
+  iDestruct "inv_t" as "[fail|#inv]".
+  { iModIntro. iSplitR; eauto. by iApply "s_t". }
+  iDestruct "counters" as "[#fail|counters]".
+  { iModIntro. iSplitR; eauto. by iApply "s_t". }
+  iDestruct "inv" as "(%si & %rl'' & %m' & %t' & %e_k & %e_t & p_ts & inv)".
+  move/term_of_senc_key_inj/session_agree: e_k => <- {si}.
+  case/Spec.of_list_inj: e_t => -> e_m <- {rl'} in ne *.
+  have <-: m = m' by lia.
+  have {ne} -> : rl'' = swap_role (cs_role cs).
+    rewrite /repr_role in ne.
+    case: rl'' (cs_role cs) => [] [] /= in ne *; congruence.
+  iMod (counters_recv with "counters inv recv") as "[counters inv_t]".
+  iMod (lc_fupd_elim_later with "c1 inv_t") as "inv_t".
+  iModIntro. iSplitR; eauto. iRight. by iFrame. }
+rewrite or_sep2. iDestruct "inv" as "[counters inv_t]".
+wp_pures. iModIntro. iRight. iExists _. iSplit => //.
+iIntros "post". iApply "post". iFrame. by eauto 10.
+Qed.
+
+Lemma wp_free kI kR φ rl cs :
+  {{{ connected kI kR φ rl cs }}}
+    impl.free (repr cs)
+  {{{ RET #(); True }}}.
+Proof.
+iIntros "%Φ conn post".
+iDestruct "conn" as "(? & ? & ? & ? & ? & % & % & ts & ?)".
+rewrite !array_cons array_nil.
+iDestruct "ts" as "(sent & recv & _)".
+wp_lam; wp_pures.
+wp_free. wp_pures.
+wp_free.
+by iApply "post".
+Qed.
+
+End Proofs.
